Add corrupted states to attacker knowledge

src/DY.Core.Attacker.Knowledge.fst
@@ -4,6 +4,8 @@ open DY.Core.Bytes.Type
 open DY.Core.Bytes
 open DY.Core.Trace.Type
 open DY.Core.Trace.Invariant
+open DY.Core.Label.Type
+open DY.Core.Label
 
 #set-options "--fuel 1 --ifuel 0"
 
@@ -12,6 +14,10 @@ let rec attacker_knows_aux step tr msg =
   if step = 0 then (
     (
       msg_sent_on_network tr msg
+    ) \/ (
+      exists prin sess_id.
+        was_corrupt tr prin sess_id /\
+        state_was_set tr prin sess_id msg
     ) \/ (
       exists lit.
         msg == literal_to_bytes lit
@@ -97,47 +103,62 @@ val move_requires_4
 let move_requires_4 #a #b #c #d #p #q pf x y z w =
   introduce p x y z w ==> q x y z w with _. pf x y z w
 
+val corrupted_state_is_publishable:
+  preds:protocol_predicates ->
+  tr:trace -> prin:principal -> sess_id:nat -> content:bytes ->
+  Lemma
+  (requires
+    was_corrupt tr prin sess_id /\
+    state_was_set tr prin sess_id content /\
+    trace_invariant preds tr
+  )
+  (ensures is_publishable preds.pr tr content)
+let corrupted_state_is_publishable preds tr prin sess_id content =
+  state_is_knowable_by preds tr prin sess_id content
+
 #push-options "--z3rlimit 25"
 val attacker_only_knows_publishable_values_aux:
-  preds:protocol_preds ->
+  preds:protocol_predicates ->
   step:nat -> tr:trace -> msg:bytes ->
   Lemma
   (requires
     trace_invariant preds tr /\
     attacker_knows_aux step tr msg
   )
-  (ensures is_publishable preds tr msg)
+  (ensures is_publishable preds.pr tr msg)
 let rec attacker_only_knows_publishable_values_aux preds step tr msg =
   if step = 0 then (
     FStar.Classical.forall_intro   (FStar.Classical.move_requires   (msg_sent_on_network_are_publishable preds tr));
-    FStar.Classical.forall_intro   (FStar.Classical.move_requires   (literal_to_bytes_is_publishable preds tr))
+    FStar.Classical.forall_intro   (FStar.Classical.move_requires   (msg_sent_on_network_are_publishable preds tr));
+    FStar.Classical.forall_intro_3 (FStar.Classical.move_requires_3 (corrupted_state_is_publishable preds tr));
+    FStar.Classical.forall_intro   (FStar.Classical.move_requires   (literal_to_bytes_is_publishable preds.pr tr))
   ) else (
     FStar.Classical.forall_intro   (FStar.Classical.move_requires   (attacker_only_knows_publishable_values_aux preds (step-1) tr));
-    FStar.Classical.forall_intro_2 (FStar.Classical.move_requires_2 (concat_preserves_publishability preds tr));
-    FStar.Classical.forall_intro_2 (FStar.Classical.move_requires_2 (split_preserves_publishability preds tr));
-    FStar.Classical.forall_intro_4 (                move_requires_4 (aead_enc_preserves_publishability preds tr));
-    FStar.Classical.forall_intro_4 (                move_requires_4 (aead_dec_preserves_publishability preds tr));
-    FStar.Classical.forall_intro   (FStar.Classical.move_requires   (pk_preserves_publishability preds tr));
-    FStar.Classical.forall_intro_3 (FStar.Classical.move_requires_3 (pk_enc_preserves_publishability preds tr));
-    FStar.Classical.forall_intro_2 (FStar.Classical.move_requires_2 (pk_dec_preserves_publishability preds tr));
-    FStar.Classical.forall_intro   (FStar.Classical.move_requires   (vk_preserves_publishability preds tr));
-    FStar.Classical.forall_intro_3 (FStar.Classical.move_requires_3 (sign_preserves_publishability preds tr));
+    FStar.Classical.forall_intro_2 (FStar.Classical.move_requires_2 (concat_preserves_publishability preds.pr tr));
+    FStar.Classical.forall_intro_2 (FStar.Classical.move_requires_2 (split_preserves_publishability preds.pr tr));
+    FStar.Classical.forall_intro_4 (                move_requires_4 (aead_enc_preserves_publishability preds.pr tr));
+    FStar.Classical.forall_intro_4 (                move_requires_4 (aead_dec_preserves_publishability preds.pr tr));
+    FStar.Classical.forall_intro   (FStar.Classical.move_requires   (pk_preserves_publishability preds.pr tr));
+    FStar.Classical.forall_intro_3 (FStar.Classical.move_requires_3 (pk_enc_preserves_publishability preds.pr tr));
+    FStar.Classical.forall_intro_2 (FStar.Classical.move_requires_2 (pk_dec_preserves_publishability preds.pr tr));
+    FStar.Classical.forall_intro   (FStar.Classical.move_requires   (vk_preserves_publishability preds.pr tr));
+    FStar.Classical.forall_intro_3 (FStar.Classical.move_requires_3 (sign_preserves_publishability preds.pr tr));
     ()
   )
 #pop-options
 
 val attacker_only_knows_publishable_values:
-  preds:protocol_preds ->
+  preds:protocol_predicates ->
   tr:trace -> msg:bytes ->
   Lemma
   (requires
     trace_invariant preds tr /\
     attacker_knows tr msg
   )
-  (ensures is_publishable preds tr msg)
+  (ensures is_publishable preds.pr tr msg)
 let attacker_only_knows_publishable_values preds tr msg =
   eliminate exists step. attacker_knows_aux step tr msg
-  returns is_publishable preds tr msg
+  returns is_publishable preds.pr tr msg
   with _. (
     attacker_only_knows_publishable_values_aux preds step tr msg
   )
